\section{基本求导公式}

\begin{multicols}{2}
    \begin{spacing}{\hangju}
        \noindent $(x^k)' = kx^{k-1}$

        \noindent $(\ln x)' = \frac{1}{x} \quad (x > 0)$

        \noindent $(e^x)' = e^x$

        \noindent $(a^x)' = a^x\ln{a} \quad (a > 0, a \neq 1)$

        \noindent $(\sin{x})' = \cos{x}$

        \noindent $(\cos{x})' = -\sin{x}$

        \noindent $(\tan{x})' = \sec^2{x}$

        \noindent $(\cot{x})' = -\csc^2{x}$

        \noindent $(\sec{x})' = \sec{x}\tan{x}$

        \noindent $(\csc{x})' = -\csc{x}\cot{x}$

        \noindent $(\ln{\left| \cos{x} \right|})' = -\tan{x}$

        \noindent $(\ln{\left| \sec{x} + \tan{x} \right|})' = \sec{x}$

        \noindent $(\ln{\left| \csc{x} - \cot{x} \right|})' = -\csc{x}$

        \noindent $(\arcsin{x})' = \frac{1}{\sqrt{1 + x^2}}$

        \noindent $(\arccos{x})' = \frac{-1}{\sqrt{1 - x^2}}$

        \noindent $(\arctan{x})' = \frac{1}{1 + x^2}$

        \noindent $( \arccot{x})' = \frac{-1}{1 + x^2}$

        \noindent $[\ln{(x + \sqrt{x^2 + a^2})}]' = \frac{1}{\sqrt{x^2 + a^2}}$

        \noindent $[\ln{(x + \sqrt{x^2 - a^2})}]' = \frac{1}{\sqrt{x^2 - a^2}}$
    \end{spacing}
\end{multicols}

